Makefile
@@ -1,0 +1,11 @@
+# Makefile
+
+COQC= coqc -Q . Elo
+
+main:
+	$(COQC) Array.v
+	$(COQC) Map.v
+	$(COQC) Core0.v
+
+clean:
+	rm -f *.vo *.vok *.vos *.glob
